Hoare/Hoare.thy
@@ -1,0 +1,290 @@
+theory Hoare imports 
+ "../Syntax/Gensyn" "../Syntax/Gensyn_Descend" "../Mergeable/Mergeable"
+ "../Semantics/Semantics" "../Semantics/Semantics_Facts"
+begin
+
+(* A simple implementation of primitives for a (sound) partial-correctness 
+ * Hoare logic on top of the general Gazelle semantics.
+ * This model of Hoare logic is based on the CPS-flavored version described in
+ * _Program Logics for Certified Compilers_ and _Separation Logic for Small-Step Cminor_
+ *)
+
+definition imm_safe :: "('syn, 'mstate) semc \<Rightarrow> ('syn, 'mstate) control  \<Rightarrow> bool" where
+"imm_safe gs m \<equiv>
+ ((cont m = Inl []) \<or>
+  (\<exists> m' . sem_step_p gs m m'))"
+
+lemma imm_safeI_Done :
+  assumes H : "cont m = Inl []"
+  shows "imm_safe gs m" using H
+  unfolding imm_safe_def by auto
+
+lemma imm_safeI_Step :
+  assumes H : "sem_step_p gs m m'"
+  shows "imm_safe gs m" using H
+  unfolding imm_safe_def
+  by(cases m'; auto)
+
+lemma imm_safeD :
+  assumes H : "imm_safe gs m"
+  shows "((cont m = Inl []) \<or>
+  (\<exists> m' . sem_step_p gs m m'))" using H
+  unfolding imm_safe_def by (auto)
+
+(* Safe means we terminate or diverge (partial correctness) *)
+definition safe :: "('syn, 'mstate) semc \<Rightarrow> ('syn, 'mstate) control \<Rightarrow> bool" where
+"safe gs m \<equiv>
+  (\<forall> m' . sem_exec_p gs m m' \<longrightarrow> imm_safe gs m')"
+
+lemma safeI [intro]:
+  assumes H : "\<And> m' . sem_exec_p gs m m' \<Longrightarrow> imm_safe gs m'"
+  shows "safe gs m" using H unfolding safe_def
+  by auto
+
+lemma safeD :
+  assumes H : "safe gs m"
+  assumes Hx : "sem_exec_p gs m m'"
+  shows "imm_safe gs m'" using H Hx
+  unfolding safe_def by blast
+
+(* Guarded: if we start in a state satisfying P, we are safe *)
+definition guarded :: "('syn, 'mstate) semc \<Rightarrow> ('mstate \<Rightarrow> bool) \<Rightarrow> 'syn gensyn list \<Rightarrow> bool"
+("|_| {_} _" [200, 202, 204])
+ where
+"guarded gs P c =
+  (\<forall> m . P (payload m) \<longrightarrow> cont m = Inl c \<longrightarrow> safe gs m)"
+
+lemma guardedI [intro] :
+  assumes H : "\<And> m . P (payload m) \<Longrightarrow> cont m = Inl c \<Longrightarrow> safe gs m"
+  shows "guarded gs P c" using H
+  unfolding guarded_def
+  by auto
+
+lemma guardedD :
+  assumes H : "guarded gs P c"
+  assumes HP : "P (payload m)"
+  assumes Hcont : "cont m = Inl c"
+  shows "safe gs m" using assms
+  unfolding guarded_def by blast
+
+(* Hoare triple definition:
+ * For any tail c' that is safe under condition Q (the postcondition of the triple),
+ * the program c followed by the tail c' will be safe under P (the precondition)
+ *)
+definition HT :: "('syn, 'mstate) semc \<Rightarrow> ('mstate \<Rightarrow> bool) \<Rightarrow> 'syn gensyn list \<Rightarrow> ('mstate \<Rightarrow> bool)\<Rightarrow> bool" 
+  ("|_| {-_-} _ {-_-}" [206, 208, 210])
+  where
+"HT gs P c Q =
+  (\<forall> c' .  |gs| {Q} (c') \<longrightarrow> |gs| {P} (c @ c'))"
+
+lemma HTI [intro] :
+  assumes H : "\<And> c' . |gs| {Q} (c') \<Longrightarrow> |gs| {P} (c @ c')"
+  shows "HT gs P c Q" using H unfolding HT_def
+  by auto
+
+lemma HTE [elim]:
+  assumes H : "HT gs P c Q"
+  assumes H' : "|gs| {Q} c'"
+  shows "|gs| {P} (c@c')" using assms
+  unfolding HT_def
+  by auto
+
+lemma HConseq :
+  assumes H : "|gs| {- P' -} c {-Q'-}"
+  assumes H' : "\<And> st . P st \<Longrightarrow> P' st"
+  assumes H'' : "\<And> st . Q' st \<Longrightarrow> Q st"
+  shows "|gs| {-P-} c {-Q-}"
+proof(rule HTI)
+  fix c'
+  assume Exec : "|gs| {Q} c'"
+
+  then have Exec' : "|gs| {Q'} c'"
+    unfolding guarded_def using H'' by blast
+
+  then have Exec'' :"|gs| {P'} (c@c')"
+    using HTE[OF H Exec'] by auto
+
+  then show "|gs| {P} (c @ c')"
+    unfolding guarded_def using H' by blast
+qed
+
+(* Lifting for non-control, single-step instructions *)
+(* TODO: this proof needs to be fixed *)
+(*
+lemma HStep : 
+  assumes H : "(! sem ) % {{P o payload}} c {{Q o payload}}"
+  assumes Hgs : "s_sem gs = sem"
+  shows "|gs| {-P-} [G c l] {-Q-}" 
+proof(rule HTI)
+  fix c'
+  assume Exec : "|gs| {Q} c'"
+
+  show "|gs| {P} [G c l] @ c'"
+  proof(rule guardedI)
+    fix m :: "('a, 'b) control"
+
+    assume P : "P (payload m)"
+    obtain ms mm mc where M: "m = (mc, mm, ms)" and P' : "P ms"
+      using P by (cases m; auto)
+
+    assume Cont : "s_cont m = Inl ([G c l] @ c')"
+
+    have Q: "Q (payload (s_sem gs c m))"
+      using H P M unfolding semprop2_def VT_def Hgs
+      by(auto)
+
+    have "s_cont (sem.s_sem gs c m) = Inl c' " using Hgs
+      apply(auto simp add: s_cont_def split: prod.splits md_prio.splits option.splits md_triv.splits)
+
+(* *)
+(* idea: sem will only modify the payload. *)
+    show "safe gs m" using guardedD[OF Exec Q]
+
+    show "safe gs m"
+    proof(rule safeI)
+      fix m'
+      assume Exec' : "sem_exec_p gs m m'"
+      show "imm_safe gs m'"
+
+      proof(cases "s_cont m'")
+        case (Inr bad)
+        then have False using Cont by auto
+        case Nil
+        then show ?thesis unfolding imm_safe_def by auto
+      next
+        case (Cons a list)
+        then show ?thesis using Exec' unfolding sem_exec_p_def imm_safe_def sem_step_p_eq sem_step_def
+          by(cases m; auto)
+      qed
+    qed
+  qed
+qed
+*)
+
+(* sequencing lemma *)
+lemma HCat :
+  assumes H : "|gs| {- P1 -} c1 {- P2 -}"
+  assumes H' : "|gs| {- P2 -} c2 {- P3 -}"
+  shows "|gs| {- P1 -} (c1 @ c2) {- P3 -}"
+proof(rule HTI)
+  fix c'
+  assume HP3 : "|gs| {P3} c'"
+
+  have P2_cont : "|gs| {P2} (c2 @ c')"
+    using HTE[OF H' HP3]
+    by auto
+
+  show "|gs| {P1} ((c1 @ c2) @ c')"
+    using HTE[OF H P2_cont]
+    unfolding append_assoc
+    by auto
+qed
+
+lemma diverges_safe :
+  assumes H : "diverges gs st"
+  shows "safe gs st" using H
+  unfolding diverges_def safe_def imm_safe_def by blast
+
+lemma guard_emp :
+  "|gs| {P} []"
+proof
+  fix m :: "('a, 'b) control"
+  assume H : "P (payload m)"
+
+  assume Hc : "cont m = Inl []"
+
+  show "safe gs m"
+  proof
+    fix m'
+
+    assume Exec : "sem_exec_p gs m m'"
+
+    hence Exec' : "rtranclp (sem_step_p gs) m m'"
+      unfolding sem_exec_p_def by auto
+
+    have Nostep : "(\<And>x1'. sem_step_p gs m x1' \<Longrightarrow> False)"
+      unfolding sem_step_p_eq using Hc
+      by(simp add: sem_step_def)
+
+    have Meq : "m = m'"
+      using rtranclp_nostep[OF sem_step_determ Exec' Nostep]
+      by auto
+
+    show "imm_safe gs m'"
+      using Hc
+      unfolding Meq imm_safe_def
+      by blast
+  qed
+qed
+
+lemma rtranclp_paths_step :
+  assumes H0 : "determ R"
+  assumes H1 : "R\<^sup>*\<^sup>* x1 y"
+  assumes H2 : "R x1 x2"
+  shows "(x1 = y \<or> R\<^sup>*\<^sup>* x2 y)" using H1 H2
+proof(induction arbitrary: x2 rule:rtranclp_induct)
+  case base
+  then show ?case by auto
+next
+  case (step nxt last)
+
+  have Opts : "x1 = nxt \<or> R\<^sup>*\<^sup>* x2 nxt"
+    using step.IH[OF step.prems(1)] by auto
+
+  then show ?case
+  proof(cases "x1 = nxt")
+    case True
+
+    then have X1alt : "R x1 last" 
+      using step.hyps by auto
+
+    then have X2alt : "x2 = last"
+      using determE[OF H0 X1alt step.prems(1)]
+      by auto
+
+    hence "R\<^sup>*\<^sup>* x2 last"
+      by auto
+
+    thus ?thesis by auto
+  next
+    case False
+
+    then have False' : "R\<^sup>*\<^sup>* x2 nxt" using Opts by auto
+
+    show ?thesis using rtranclp.intros(2)[OF False' step.hyps(2)]
+      by auto
+  qed
+qed
+
+lemma safe_exec_safe :
+  assumes H1 : "safe gs m"
+  assumes H2 : "sem_exec_p gs m m'"
+  shows "safe gs m'" using H2 H1 unfolding sem_exec_p_def
+proof(induction rule: rtranclp_induct)
+  case base
+  then show ?case by blast
+next
+  case (step y z)
+
+  have SafeY: "safe gs y"
+    using step.prems step.IH by blast
+
+  show ?case
+  proof
+    fix z'
+    assume "sem_exec_p gs z z'"
+
+    hence Exec1 : "(sem_step_p gs)\<^sup>*\<^sup>* z z'" 
+      unfolding sem_exec_p_def
+      by simp
+
+    have ExecFull : "sem_exec_p gs y z'"
+      using step.hyps(2) Exec1
+      by auto
+
+    show "imm_safe gs z'" using safeD[OF SafeY ExecFull] by simp
+  qed
+qed
+
+      
+end
